$$E_\pm(\textbf{r},t)=\frac{\varepsilon_{\pm}(\textbf{r})}{2}e^{-i(\omega{t}\mp{kz})}+c.c.$$
$by∇⋅E=0$
$$∇⋅E_\pm(\textbf{r},t)=∇⋅[\frac{\varepsilon_{\pm}(\textbf{r})}{2}e^{-i(\omega{t}\mp{kz})}+c.c.]=0$$
$$∇⋅[\varepsilon_{\pm}(\textbf{r})e^{-i(\omega{t}\mp{kz})}]=(\frac{\partial}{\partial_x}+\frac{\partial}{\partial_y}+\frac{\partial}{\partial_z})\cdot(\varepsilon_x+\varepsilon_y+\varepsilon_z)\cdot(e^{-i(\omega{t}\mp{kz})})$$
$$(e^{-i(\omega{t}\mp{kz})})\cdot(\frac{\partial\varepsilon_x}{\partial_x})+(e^{-i(\omega{t}\mp{kz})})\cdot(\frac{\partial\varepsilon_y}{\partial_y})+(e^{-i(\omega{t}\mp{kz})})\cdot(\frac{\partial\varepsilon_z}{\partial_z})+\varepsilon_z\cdot(-ik)e^{-i(\omega{t}\mp{kz})}=0$$
where $\frac{\partial\epsilon_z}{\partial_z}\rightarrow0$ ,  $(-ik)\rightarrow(\frac{k}{i})$ and 同除 $(e^{-i(\omega{t}\mp{kz})})$
$$(\frac{\partial\varepsilon_x}{\partial_x})+(\frac{\partial\varepsilon_y}{\partial_y})+\varepsilon_z\cdot(\frac{k}{i})e^{-i(\omega{t}\mp{kz})}=0$$
$$\varepsilon_{z}=-\frac{i}{k}(\frac{\partial{\varepsilon_{x}}}{\partial_x}+\frac{\partial{\varepsilon_{y}}}{\partial_y})$$
$$\varepsilon_{\pm,z}=\mp\frac{i}{k}(\frac{\partial{\varepsilon_{\pm,x}}}{\partial_x}+\frac{\partial{\varepsilon_{\pm,y}}}{\partial_y})$$

